\subsection{Coequalizer}
\label{sec:coequalizer}

Given two 1-types $A$ and $B$ and two functions $f , g: A \to B$, the
coequalizer of $f$ and $g$ is given by the following HIT:
\begin{lstlisting}[mathescape=true]
Inductive $\coequalizer f g$ :=
| $\coequalizerbase$ : $B \rightarrow \coequalizer f g$
| $\coequalizerglue$ : $\depprod{(x : A)}{\coequalizerbase(f(x)) = \coequalizerbase(g(x))}$
\end{lstlisting}

The signature of the coequalizer of $f$ and $g$ is:
\begin{itemize}
\item $\pointconstr[\coequalizer f g] = \constantP{B}$;
\item $\pathlabel[\coequalizer f g] = \unit$, and for its unique inhabitant take $\patharg[\coequalizer f g] = \constantP{A}$ and endpoints
  \[
  \pathleft[\coequalizer f g] = \comp{\fmap(f)}{\constr}, \quad
  \pathright[\coequalizer f g] = \comp{\fmap(g)}{\constr}; 
  \]
\item $\homotlabel[\coequalizer f g]$ is the empty type.
\end{itemize}

\subsection{Coequifier}
\label{sec:coequifier}

Assume two 1-types $A$ and $B$, two functions $f , g: A \to B$ and two
homotopies $p$ and $q$ between $f$ and $g$. The coequifier of $p$ and
$q$ is given by the following HIT:
\begin{lstlisting}[mathescape=true]
Inductive $\coequifier p q$ :=
| $\coequifierbase$ : $B \rightarrow \coequifier f g$
| $\coequifierglue$ : $\depprod{(x : A)}{\ap {\coequifierbase}{(p(x))} = \ap {\coequifierbase}{(q(x))}}$
\end{lstlisting}

The signature of the coequifier of $p$ and $q$ is:
\begin{itemize}
\item $\pointconstr[\coequifier f g] = \constantP{B}$;
\item $\pathlabel[\coequifier f g]$ is the empty type; 
\item $\homotlabel[\coequifier f g] = \unit$, and take 
  $\homotpointarg[\coequifier f g] = \constantP{A}$.
  The homotopy constructor $\coequifierglue$ does not have path arguments, so we take  
  $\homotpathtarg[\coequifier f g] = \constantP{\unit}$ and
  $\pathargleft[\coequifier f g] = \pathargright[\coequifier f g] = \Ce(\unitt)$.
  The endpoints $\homotpathleft[\coequifier f g]$ and $\homotpathright[\coequifier f g]$ are
  \[
  \homotpathleft[\coequifier f g] = \comp{\fmap(f)}{\constr}, \quad
  \homotpathright[\coequifier f g] = \comp{\fmap(g)}{\constr},
  \]
  and the left and right homotopy endpoints are
  \[
  \hap{(\idtoH(\funextsec(p)))}, \quad
  \hap{(\idtoH(\funextsec(q)))}.
  \]
\end{itemize}


\subsection{Group Quotient}
\label{sec:group_quotient}

Let $G$ be a group with unit $e$ and multiplication $*$. The group
quotient of $G$ is the following HIT:
\begin{lstlisting}[mathescape=true]
Inductive $\groupquot G$ :=
| $\groupquotbase$ : $\groupquot G$
| $\groupquotloop$ : $G \rightarrow \groupquotbase = \groupquotbase$
| $\groupquotloope$ : $\groupquotloop(e)= \refl \groupquotbase$
| $\groupquotloopm$ : $\depprod{(x,y : G)}{\groupquotloop(x * y)= \concat{\groupquotloop(x)}{\groupquotloop(y)}}$
\end{lstlisting}


Signature for the group quotient

\subsection{Monoidal Object}
\label{sec:monoidal_object}

The monoidal object is defined by the following HIT:
\begin{lstlisting}[mathescape=true]
Inductive $\monobj$ :=
| $\monobjunit$ : $\monobj$
| $\monobjtensor$ : $\monobj \rightarrow \monobj \rightarrow \monobj$
| $\monobjlambda$ : $\depprod{(x : \monobj)}{\monobjtensor(\monobjunit,x) = x}$
| $\monobjrho$ : $\depprod{(x : \monobj)}{\monobjtensor(x,\monobjunit) = x}$
| $\monobjalpha$ : $\depprod{(x ,y,z: \monobj)}{\monobjtensor(x,(\monobjtensor(y,z)))=\monobjtensor(\monobjtensor(x,y),z)}$
| $\monobjtr$ : $\depprod{(x,y : \monobj)}{\ap{(\Lam z. \monobjtensor(x,z))}{(\monobjlambda(y))}} = \concat{\monobjalpha(x,\monobjunit,y)}{\ap{(\Lam z. \monobjtensor(z,y))}{(\monobjrho(x))}}$
| $\monobjpent$ : $\depprod{(w,x,y,z : \monobj)}{}$
    $\concat{\monobjalpha(w,x,\monobjtensor(y,z))}{\monobjalpha(\monobjtensor(w,x),y,z)}=\concat{\ap{(\Lam v. \monobjtensor(w,v))}{(\monobjalpha(x,y,z))}}{\concat{\monobjalpha(w,\monobjtensor(x,y),z)}{\ap{(\Lam v. \monobjtensor(v,z))}{(\monobjalpha(w,x,y))}}}$
\end{lstlisting}

Signature for the monoidal object

\subsection{Coherent Group}
\label{sec:coeherent_group}

The coherent group is defined by the following HIT:
\begin{lstlisting}[mathescape=true]
Inductive $\cohgroup$ :=
| $\cohgroupunit$ : $\cohgroup$
| $\cohgrouptensor$ : $\cohgroup \rightarrow \cohgroup \rightarrow \cohgroup$
| $\cohgroupinv$ : $\cohgroup \rightarrow \cohgroup$
| $\cohgrouplambda$ : $\depprod{(x : \cohgroup)}{\cohgrouptensor(\cohgroupunit,x) = x}$
| $\cohgrouprho$ : $\depprod{(x : \cohgroup)}{\cohgrouptensor(x,\cohgroupunit) = x}$
| $\cohgroupalpha$ : $\depprod{(x ,y,z: \cohgroup)}{\cohgrouptensor(x,(\cohgrouptensor(y,z)))=\cohgrouptensor(\cohgrouptensor(x,y),z)}$
| $\cohgrouplinv$ : $\depprod{(x : \cohgroup)}{\cohgrouptensor(\cohgroupinv(x),x) = \cohgroupunit}$
| $\cohgrouprinv$ : $\depprod{(x : \cohgroup)}{\cohgroupunit = \cohgrouptensor(x,\cohgroupinv(x))}$
| $\cohgrouptr$ : $\depprod{(x,y : \cohgroup)}{\ap{(\Lam z. \cohgrouptensor(x,z))}{(\cohgrouplambda(y))}} = \concat{\cohgroupalpha(x,\cohgroupunit,y)}{\ap{(\Lam z. \cohgrouptensor(z,y))}{(\cohgrouprho(x))}}$
| $\cohgrouppent$ : $\depprod{(w,x,y,z : \cohgroup)}{}$
    $\concat{\cohgroupalpha(w,x,\cohgrouptensor(y,z))}{\cohgroupalpha(\cohgrouptensor(w,x),y,z)}=\concat{\ap{(\Lam v. \cohgrouptensor(w,v))}{(\cohgroupalpha(x,y,z))}}{\concat{\cohgroupalpha(w,\cohgrouptensor(x,y),z)}{\ap{(\Lam v. \cohgrouptensor(v,z))}{(\cohgroupalpha(w,x,y))}}}$
| $\cohgroupinvadjtrl$ : $\depprod{(x : \cohgroup)}{\concat{\ap{(\Lam z. \cohgrouptensor(z,x))}{(\cohgrouprinv(x))}}{\concat{\inverse{(\cohgroupalpha(x,\cohgroupinv(x),x))}}{\ap{(\Lam z. \cohgrouptensor(x,z))}{(\cohgrouplinv(x))}}}=\concat{\cohgrouplambda(x)}{\inverse{(\cohgrouprho(x))}}}$
| $\cohgroupinvadjtrr$ : $\depprod{(x : \cohgroup)}{\concat{\ap{(\Lam z. \cohgrouptensor(\cohgroupinv(x),z))}{(\cohgrouprinv(x))}}{\concat{\cohgroupalpha(\cohgroupinv(x),x,\cohgroupinv(x))}{\ap{(\Lam z. \cohgrouptensor(z,\cohgroupinv(x)))}{(\cohgrouplinv(x))}}}=\concat{\cohgrouprho(\cohgroupinv(x))}{\inverse{(\cohgrouplambda(\cohgroupinv(x)))}}}$
\end{lstlisting}





Signature for the coherent group
